Proved Ludo's conjecture

theories/Interp/Sched.v
@@ -39,11 +39,407 @@ Definition round_robin {E} : ctree E ~> stateT nat (ctree E).
                 *)
                match n as n' return (ctree E (nat * fin n')) with
                | O => CTree.stuckI
-               | S n => (Ret (S m, @Fin.of_nat_lt (Nat.modulo m (S n)) _ _))
+               | 1 => Ret (m, Fin.F1)
+               | S (S n) => (Ret (S m, @Fin.of_nat_lt (Nat.modulo m (S (S n))) _ _))
                end
          )).
   apply (NPeano.Nat.mod_upper_bound).
   auto with arith.
 Defined.
 
+(* TODO:
+Can we do something with a stream?
+One round robin per arity?
+Random scheduler on the OCaml side?
+Fairness? Too low level here I think? Maybe at the level of Imp.
+Prove that the original computation simulates the scheduled one?
+*)
+
+
+(* TODO: move, use globally? *)
+Notation ChoiceVF := (ChoiceF true).
+Notation ChoiceIF := (ChoiceF false).
+
+Definition guarded_form {E X} (t : ctree E X) : ctree E X :=
+	CTree.iter (fun t =>
+				        match observe t with
+				        | RetF r => ret (inr r)
+				        | ChoiceIF n k =>
+                    ChoiceI n (fun x => Ret (inl (k x)))
+				        | ChoiceVF n k =>
+                    ChoiceI n (fun x => TauV (Ret (inl (k x))))
+				        | VisF e k => bind (mtrigger _ e) (fun x => Ret (inl (k x)))
+				        end) t.
+
+Lemma unfold_guarded_form {E X} (t : ctree E X) :
+  guarded_form t ≅
+  match observe t with
+	| RetF r => ret r
+	| ChoiceIF n k =>
+      ChoiceI n (fun x => TauI (guarded_form (k x)))
+	| ChoiceVF n k =>
+      ChoiceI n (fun x => TauV (TauI (guarded_form (k x))))
+	| VisF e k => bind (mtrigger _ e) (fun x => TauI (guarded_form (k x)))
+	end.
+Proof.
+  unfold guarded_form at 1.
+  rewrite unfold_iter.
+  desobs t; cbn.
+  - now rewrite bind_ret_l.
+  - unfold mtrigger; rewrite bind_bind, !bind_trigger.
+    step; constructor; intros ?.
+    rewrite bind_ret_l.
+    reflexivity.
+  - destruct vis.
+    + rewrite bind_choice.
+      step; constructor; intros ?.
+      rewrite bind_tauV; step; constructor; intros ?.
+      rewrite bind_ret_l.
+      step; constructor; auto.
+    + rewrite bind_choice.
+      step; constructor; intros ?.
+      rewrite bind_ret_l.
+      step; constructor; auto.
+Qed.
+
+(* TODO: export globally? *)
+From RelationAlgebra Require Import
+     rel srel.
+
+(* TODO: think about all this stuff and move it *)
+Lemma step_sbisim_vis_gen {E X Y} (e : E X) (k k' : X -> ctree E Y) (R : rel _ _) :
+  (Proper (equ eq ==> equ eq ==> Basics.impl) R) ->
+  (forall x, R (k x) (k' x)) ->
+  sb R (Vis e k) (Vis e k').
+Proof.
+  intros PR EQs.
+  split; intros ? ? TR; inv_trans; subst.
+  all: cbn; eexists; etrans; rewrite EQ; auto.
+Qed.
+
+Lemma step_sbisim_vis {E X Y} (e : E X) (k k' : X -> ctree E Y) (R : rel _ _) :
+  (forall x, (st R) (k x) (k' x)) ->
+  sb (st R) (Vis e k) (Vis e k').
+Proof.
+  apply step_sbisim_vis_gen.
+  typeclasses eauto.
+Qed.
+
+Lemma step_sbisim_tauV_gen {E X} (t t' : ctree E X) (R : rel _ _) :
+  (Proper (equ eq ==> equ eq ==> Basics.impl) R) ->
+  (R t t') ->
+  sb R (TauV t) (TauV t').
+Proof.
+  intros PR EQs.
+  split; intros ? ? TR; inv_trans; subst.
+  all: cbn; eexists; etrans; rewrite EQ; auto.
+Qed.
+
+Lemma step_sbisim_tauV {E X} (t t' : ctree E X) (R : rel _ _) :
+  (st R t t') ->
+  sb (st R) (TauV t) (TauV t').
+Proof.
+  apply step_sbisim_tauV_gen.
+  typeclasses eauto.
+Qed.
+
+Ltac svis  := apply step_sbisim_vis.
+Ltac stauv := apply step_sbisim_tauV.
+Ltac sstep := svis || stauv.
+
+Lemma step_sbisim_choiceI_gen {E X} n m (k : fin n -> ctree E X) (k' : fin m -> ctree E X) (R : rel _ _) :
+  (forall x, exists y, sb R (k x) (k' y)) ->
+  (forall y, exists x, sb R (k x) (k' y)) ->
+  sb R (ChoiceI n k) (ChoiceI m k').
+Proof.
+  intros EQs1 EQs2.
+  split; intros ? ? TR; inv_trans; subst.
+  - destruct (EQs1 n0) as [x [F _]]; cbn in F.
+    apply F in TR; destruct TR as [u' TR' EQ'].
+    eexists.
+    eapply trans_choiceI with (x := x); [|reflexivity].
+    eauto.
+    eauto.
+  - destruct (EQs2 m0) as [x [_ B]]; cbn in B.
+    apply B in TR; destruct TR as [u' TR' EQ'].
+    eexists.
+    eapply trans_choiceI with (x := x); [|reflexivity].
+    eauto.
+    eauto.
+Qed.
+
+Lemma step_sbisim_choiceI_id {E X} n (k k' : fin n -> ctree E X) (R : rel _ _) :
+  (forall x, sb R (k x) (k' x)) ->
+  sb R (ChoiceI n k) (ChoiceI n k').
+Proof.
+  intros; apply step_sbisim_choiceI_gen.
+  intros x; exists x; apply H.
+  intros x; exists x; apply H.
+Qed.
+
+Lemma step_sbisim_choiceI_id' {E X} n (k k' : fin n -> ctree E X)  :
+  (forall x, (k x) ~ (k' x)) ->
+  (ChoiceI n k) ~ (ChoiceI n k').
+Proof.
+  intros.
+  step.
+  eapply step_sbisim_choiceI_id.
+  intros.
+  specialize (H x).
+  now step in H.
+Qed.
+
+Lemma foo {E X} l (t t' u : ctree E X):
+  t ~ t' ->
+  trans l t u ->
+  exists u', trans l t' u' /\ u ~ u'.
+Proof.
+  intros * EQ TR.
+  step in EQ; destruct EQ as [F _]; apply F in TR; destruct TR; eauto.
+Qed.
+
+Lemma trans_guarded_inv_strong :
+  forall {E X} (t u v : ctree E X) l,
+    (v ≅ guarded_form t \/ v ≅ TauI (guarded_form t)) ->
+    trans l v u ->
+    exists t', trans l t t'
+          /\ (u ≅ guarded_form t' \/ u ≅ TauI (guarded_form t')).
+Proof.
+  intros * EQ TR.
+  revert t EQ.
+  unfold trans in TR; repeat red in TR.
+  dependent induction TR.
+  - intros ? [EQ | EQ].
+    + rewrite ctree_eta, <- x, unfold_guarded_form in EQ.
+      setoid_rewrite (ctree_eta t).
+      desobs t; try now step in EQ; inv EQ.
+      destruct vis.
+      * pose proof equ_choice_invT _ _ EQ as [<- _].
+        apply equ_choice_invE with (x := x0) in EQ .
+        rewrite EQ in TR.
+        apply trans_tauV_inv in TR as [EQ' ->].
+        eexists; split; eauto.
+        etrans.
+
+      * pose proof equ_choice_invT _ _ EQ as [<- _].
+        apply equ_choice_invE with (x := x0) in EQ .
+        specialize (IHTR _ _ eq_refl eq_refl).
+        edestruct IHTR as (t' & ? & ?); eauto.
+        exists t'.
+        split.
+        eapply trans_choiceI with (x := x0); eauto.
+        eauto.
+
+    + rewrite ctree_eta, <- x in EQ.
+      pose proof equ_choice_invT _ _ EQ as [-> _].
+      apply equ_choice_invE with (x := x0) in EQ .
+      specialize (IHTR _ _ eq_refl eq_refl).
+      edestruct IHTR as (t' & ? & ?); eauto.
+
+  - (* G(t) ≅ ChoiceV k : absurd *)
+    intros ? [EQ | EQ].
+    + rewrite ctree_eta, <- x1, unfold_guarded_form in EQ.
+      desobs t0; try now step in EQ; inv EQ.
+      destruct vis; try now step in EQ; inv EQ.
+    + rewrite ctree_eta, <- x1 in EQ.
+      now step in EQ; inv EQ.
+
+  - (* G(t) ≅ Vis e k : t ≅ Vis e k', k x ≅ TauI (G (k' x)) *)
+    intros ? [EQ | EQ].
+    + setoid_rewrite (ctree_eta t0).
+      rewrite ctree_eta, <- x1, unfold_guarded_form in EQ.
+      rewrite (ctree_eta t), x in H.
+      clear t x.
+      desobs t0; try now step in EQ; inv EQ.
+      2:destruct vis; try now step in EQ; inv EQ.
+      cbn in *.
+      unfold mtrigger in EQ; rewrite bind_trigger in EQ.
+      pose proof equ_vis_invT _ _ _ _ EQ; subst.
+      pose proof equ_vis_invE _ _ _ _ EQ as [-> EQ'].
+      eexists; split.
+      etrans.
+      rewrite <- ctree_eta in H.
+      rewrite <- H.
+      rewrite EQ'.
+      auto.
+    + rewrite ctree_eta, <- x1 in EQ.
+      now step in EQ; inv EQ.
+
+  - (* G(t) ≅ Ret x : t ≅ Ret x *)
+    intros ? [EQ | EQ].
+    + setoid_rewrite (ctree_eta t).
+      rewrite ctree_eta, <- x0, unfold_guarded_form in EQ.
+      desobs t; try now step in EQ; inv EQ.
+      2:destruct vis; try now step in EQ; inv EQ.
+      step in EQ; inv EQ.
+      eexists; split.
+      etrans.
+      left.
+      rewrite ctree_eta, <- x, unfold_guarded_form.
+      cbn.
+      rewrite ! choiceI0_always_stuck.
+      reflexivity.
+    + rewrite ctree_eta, <- x0 in EQ.
+      now step in EQ; inv EQ.
+Qed.
+
+Lemma trans_guarded_inv :
+  forall E X (t u : ctree E X) l,
+    trans l (guarded_form t) u ->
+    exists t', trans l t t'
+          /\ u ~ guarded_form t'.
+Proof.
+  intros.
+  edestruct @trans_guarded_inv_strong as (t' & TR & EQ); [|eassumption|].
+  left; eauto.
+  exists t'; split; auto.
+  destruct EQ as [EQ |EQ]; rewrite EQ; auto.
+  rewrite sb_tauI; auto.
+Qed.
+
+Ltac fold_bind :=
+  repeat match goal with
+           |- context [CTree.subst ?k ?t] => fold (CTree.bind t k)
+         end.
+
+#[global] Instance guarded_equ E X : Proper (equ eq ==> equ eq) (@guarded_form E X).
+Proof.
+  do 2 red.
+  coinduction ? IH.
+  intros * EQ.
+  step in EQ.
+  rewrite ! unfold_guarded_form.
+  cbn.
+  inv EQ; auto.
+  - cbn.
+    constructor; intros ?.
+    fold_bind; rewrite ! bind_ret_l.
+    step; constructor; intros _.
+    auto.
+  - destruct b; cbn.
+    all: constructor; intros ?.
+    all: repeat (step; constructor; intros ?).
+    all: auto.
+Qed.
+
+(* TODO: bind simpl never globally? *)
+(* TODO: Taus without continuation? *)
+(* TODO: tactic for better stepping for equ *)
+(* TODO: tactics for better stepping for sbisim (see a couple above) *)
+(* Equality on [observe u] rewritten in [equ]? *)
+Opaque CTree.bind.
+Lemma trans_guarded_strong :
+  forall E X (t u : ctree E X) l,
+    trans l t u ->
+    exists u',
+      trans l (guarded_form t) u'
+      /\ (u' ≅ guarded_form u
+         \/ u' ≅ TauI (guarded_form u)).
+Proof.
+  intros * TR.
+  (* revert t EQ. *)
+  unfold trans in TR; repeat red in TR.
+  dependent induction TR; intros.
+  - (* destruct EQ as [EQ | EQ]. *)
+    edestruct IHTR as (u' & TR' & EQ'); eauto.
+    setoid_rewrite unfold_guarded_form at 1; rewrite <- x.
+    exists u'; split.
+    eapply trans_choiceI with (x := x0); [| reflexivity].
+    now apply trans_tauI.
+    auto.
+  - setoid_rewrite unfold_guarded_form at 1; rewrite <- x1.
+    eexists; split.
+    eapply trans_choiceI with (x := x0); [| reflexivity].
+    etrans.
+    right.
+    step; constructor; intros ?.
+    rewrite H.
+    rewrite (ctree_eta t0),x,<- ctree_eta.
+    auto.
+  - setoid_rewrite unfold_guarded_form at 1; rewrite <- x1.
+    eexists; split.
+    unfold mtrigger, ctree_trigger; cbn.
+    rewrite bind_trigger.
+    etrans.
+    right.
+    step; constructor; intros ?.
+    rewrite H.
+    rewrite (ctree_eta t0),x,<- ctree_eta.
+    auto.
+  - setoid_rewrite unfold_guarded_form at 1; rewrite <- x0.
+    eexists; split.
+    (*
+      Why do I need to cbn even if I add:
+      Hint Unfold ret Monad_ctree : trans.
+     *)
+    cbn; etrans.
+    left.
+    rewrite unfold_guarded_form, <- x; cbn.
+    now rewrite ! choiceI0_always_stuck.
+Qed.
+
+Lemma trans_guarded :
+  forall E X (t u : ctree E X) l,
+    trans l t u ->
+    exists u',
+      trans l (guarded_form t) u'
+      /\ u' ~ guarded_form u.
+Proof.
+  intros * TR.
+  edestruct trans_guarded_strong as (u' & TR' & EQ'); eauto.
+  exists u'; split; auto.
+  destruct EQ' as [EQ' | EQ']; rewrite EQ'; auto.
+  now rewrite sb_tauI.
+Qed.
+
+Lemma guarded_is_bisimilar {E X} : forall (t : ctree E X),
+    guarded_form t ~ t.
+Proof.
+  coinduction ? IH.
+  intros t.
+  rewrite (ctree_eta t) at 2.
+  rewrite unfold_guarded_form.
+  desobs t.
+  - now cbn.
+  - cbn.
+    unfold mtrigger; rewrite bind_trigger.
+    sstep; intros ?.
+    rewrite sb_tauI.
+    apply IH.
+  - destruct vis.
+    + cbn.
+      split; intros ? ? TR.
+      * inv_trans.
+        subst.
+        eexists.
+        eapply trans_choiceV with (x := n0).
+        rewrite EQ.
+        rewrite sb_tauI.
+        apply IH.
+      * cbn.
+        inv_trans; subst.
+        eexists.
+        eapply trans_choiceI with (x := n0).
+        2:etrans.
+        etrans.
+        rewrite sb_tauI.
+        rewrite EQ; apply IH.
+    + split.
+      * intros ? ? TR.
+        cbn.
+        inv_trans.
+        edestruct trans_guarded_inv as (u' & TR' & EQ'); eauto.
+        eexists.
+        eapply trans_choiceI with (x := n0); [| reflexivity].
+        eassumption.
+        rewrite EQ'; auto.
+      * cbn; intros ? ? TR.
+        inv_trans.
+        edestruct trans_guarded as (u' & TR' & EQ'); eauto.
+        eexists.
+        eapply trans_choiceI with (x := n0); [| reflexivity].
+        apply trans_tauI.
+        eauto.
+        rewrite EQ'; auto.
+Qed.
 
